theories/rules/retrieve.v
@@ -7,7 +7,7 @@ Section retrieve.
 
 Context `{vmG: !gen_VMG Σ}.
 
-Lemma hvc_retrieve_donate_nz {wi sown sacc pi sexcl i j des ptx rxp l} {spsd: gset PID}
+Lemma hvc_retrieve_donate_nz {wi sown sacc pi sexcl i j des ptx rxp l sh} {spsd: gset PID}
       ai r0 r1 wh wf (psd: list PID) :
   (* the current instruction is hvc *)
   (* the decoding of wi is correct *)
@@ -31,10 +31,374 @@ Lemma hvc_retrieve_donate_nz {wi sown sacc pi sexcl i j des ptx rxp l} {spsd: gs
   ∗ ▷ (R0 @@ i ->r r0) ∗ ▷ wh ->re false
   ∗ ▷ (R1 @@ i ->r r1) ∗ ▷ wh ->t{1}(j, wf, i, psd, Donation)
   ∗ ▷ O@i:={1}[sown] ∗ ▷ E@i:={1}[sexcl] ∗ ▷ TX@ i := ptx
-  ∗ ▷ mem_region des ptx ∗ ▷ RX@ i :=( rxp !) ∗ ▷ (∃l, mem_region l rxp ∗ ⌜ length l = length des ⌝)}}}
+  ∗ ▷ mem_region des ptx ∗ ▷ RX@ i :=( rxp !) ∗ ▷ (∃l, mem_region l rxp ∗ ⌜ length l = length des ⌝)
+  ∗ ▷ hp{ 1 }[ sh ] }}}
    ExecI @ i {{{ RET ExecI ; PC @@ i ->r (ai ^+ 1)%f ∗ ai ->a wi
   ∗ O@i:={1}[(sown ∪ spsd)] ∗ E@i:={1}[(sexcl ∪ spsd)] ∗ A@i:={1}[(sacc ∪ spsd)]
-  ∗ R0 @@ i ->r (encode_hvc_ret_code Succ) ∗ R1 @@ i ->r r1 ∗ wh ->t{1}(j, wf, i, psd, Donation)
+  ∗ R0 @@ i ->r (encode_hvc_ret_code Succ) ∗ R1 @@ i ->r r1
+  ∗ TX@ i := ptx ∗ RX@ i :=( rxp ! r1, i)
+  ∗ mem_region des ptx ∗ mem_region des rxp
+  ∗ hp{ 1 }[ sh ∪ {[wh]} ] }}}.
+Proof.
+  iIntros (Hdecodei Hinpi Hdecodef Hpiacc Hpsd Hsown Hsacc Hsexcl Hlenl Hdes Hdesl Hseq Φ).
+  iIntros "(>PC & >Hai & >HA & >Hr0 & >Hwhf & >Hr1 & >Hwh & >HO & >HE & >HTX & >Hmemr & >HRX & >HRXCont & >Hpool) HΦ".
+  iApply (sswp_lift_atomic_step ExecI); [done|].
+  iIntros (σ1) "%Hsche Hσ".
+  inversion Hsche as [Hcureq]; clear Hsche.
+  apply fin_to_nat_inj in Hcureq.
+  iModIntro.
+  iDestruct "Hσ" as "(Hcur & Hσmem & Hσreg & Hσtx & Hσrx1 & Hσrx2 & Hσowned & Hσaccess & Hσexcl & Htrans & Hσhp & %Hdisj & %Hlen & Hrcv)".
+  iDestruct ((gen_reg_valid3 i PC ai R0 r0 R1 r1 Hcureq) with "Hσreg PC Hr0 Hr1")
+    as "[%HPC [%HR0 %HR1]]"; eauto.
+  iDestruct ((gen_access_valid_addr_elem ai sacc) with "Hσaccess HA") as %Haccai; eauto.
+  { rewrite (to_pid_aligned_in_page _ pi); eauto. }
+  iDestruct ((gen_access_valid_pure sacc) with "Hσaccess HA") as %Hacc; eauto.
+  iDestruct (gen_mem_valid ai wi with "Hσmem Hai") as %Hai.
+  iDestruct (gen_trans_valid with "Hwh Htrans") as %Htrans.
+  destruct Htrans as [b Htrans].
+  iDestruct (gen_retri_valid with "Hwhf Hrcv") as %Hretri.
+  destruct Hretri as [t [Hretri1 Hretri2]].
+  iDestruct (gen_mem_valid_SepL_pure _ des with "Hσmem Hmemr") as %Hadesc.
+  { apply finz_seq_NoDup. destruct Hseq as [? [HisSome ?]]. done. }
+  iDestruct (gen_tx_valid with "HTX Hσtx") as %Htx.
+  iDestruct (gen_rx_valid_none with "HRX Hσrx2") as %Hrx2.
+  iDestruct "HRX" as "(HRX1 & HRX2)".
+  iDestruct (gen_rx_pid_valid with "HRX1 Hσrx1") as %Hrx1.
+  iDestruct ((gen_own_valid_pure sown) with "Hσowned HO") as %Hown; eauto.
+  iDestruct ((gen_excl_valid_pure sexcl) with "Hσexcl HE") as %Hexcl; eauto.
+  iDestruct ((gen_hpool_valid_elem sh) with "Hpool Hσhp") as %Hpool; eauto.
+  iSplit.
+  - (* reducible *)
+    iPureIntro.
+    apply (reducible_normal i Hvc ai wi); eauto.
+  - (* step *)
+    iModIntro.
+    iIntros (m2 σ2) "%HstepP".
+    apply (step_ExecI_normal i Hvc ai wi) in HstepP; eauto.
+    remember (exec Hvc σ1) as c2 eqn:Heqc2.
+    rewrite /exec /hvc HR0 Hdecodef /retrieve /get_transaction HR1 //= in Heqc2.
+    assert (Hlendesclt :((Z.of_nat (length des)) <= (page_size-1))%Z).
+    {
+      destruct Hseq as [? [HisSome Hltpagesize]].
+      apply (finz_plus_Z_le (of_pid ptx)); eauto.
+      apply last_addr_in_bound.
+      apply Z.leb_le.
+      destruct (((ptx ^+ length des)%f <=? (ptx ^+ (page_size - 1))%f)%Z).
+      done.
+      contradiction.
+    }
+    destruct (page_size <? r1)%Z eqn:Hr1ps; [lia|].
+    rewrite /get_tx_pid_global Hcureq Htx in Heqc2.
+    rewrite (@transaction_retrieve_descriptor_valid j wh wf l psd σ1 des ptx) /= in Heqc2; eauto.    
+    2: { rewrite Hcureq; auto. }
+    rewrite Htrans /= in Heqc2.
+    rewrite /transfer_msg /transfer_msg_unsafe Hr1ps //= /get_current_vm //= /get_vm_mail_box /get_mail_boxes //in Heqc2.
+    rewrite /get_vm_mail_box /get_mail_boxes in Htx Hrx2.
+    pose proof (surjective_pairing (σ1.1.1.1.1.2 !!! i)) as Hpair.
+    rewrite (surjective_pairing (σ1.1.1.1.1.2 !!! i).2) in Hpair.
+    rewrite Htx Hrx1 Hrx2 in Hpair.
+    rewrite //= /fill_rx /get_vm_mail_box /get_mail_boxes // /get_mail_boxes // in Heqc2.
+    rewrite Hpair //= in Heqc2.
+    destruct HstepP; subst m2 σ2; subst c2; simpl.
+    rewrite /gen_vm_interp /update_incr_PC /update_reg.
+    rewrite update_offset_PC_preserve_current_vm
+            update_access_batch_preserve_current_vm
+            update_ownership_batch_preserve_current_vm
+            update_reg_global_preserve_current_vm
+            remove_transaction_preserve_current_vm
+            fill_rx_unsafe_preserve_current_vm
+            copy_page_segment_unsafe_preserve_current_vm.
+    cbn.
+    iFrame "Hcur".
+    rewrite update_offset_PC_preserve_tx
+            update_access_batch_preserve_tx
+            update_ownership_batch_preserve_tx
+            update_reg_global_preserve_tx
+            remove_transaction_preserve_tx
+            fill_rx_unsafe_preserve_tx.
+    2 : {
+      rewrite /get_tx_pid_global /get_vm_mail_box //= /get_mail_boxes.
+    }
+    rewrite copy_page_segment_unsafe_preserve_tx.
+    rewrite /get_tx_agree.
+    iFrame "Hσtx".
+    rewrite update_offset_PC_preserve_rx1
+            update_access_batch_preserve_rx1
+            update_ownership_batch_preserve_rx1
+            update_reg_global_preserve_rx1
+            remove_transaction_preserve_rx1
+            fill_rx_unsafe_preserve_rx1.
+    rewrite copy_page_segment_unsafe_preserve_rx1.
+    iFrame "Hσrx1".
+    (* update regs *)
+    rewrite (update_offset_PC_update_PC1 _ i ai 1).
+    rewrite update_access_batch_preserve_regs update_ownership_batch_preserve_regs update_reg_global_update_reg.
+    rewrite remove_transaction_preserve_regs fill_rx_unsafe_preserve_regs copy_page_segment_unsafe_preserve_regs;
+      try solve_reg_lookup.
+    2 : {
+      exists r0.
+      rewrite get_reg_gmap_get_reg_Some.
+      rewrite /get_reg /get_reg_global /get_vm_reg_file /get_reg_files //= Hcureq /get_current_vm //= in HR0 *.
+      f_equal.
+    }
+    2 : {
+      rewrite update_access_batch_preserve_current_vm
+              update_ownership_batch_preserve_current_vm
+              update_reg_global_preserve_current_vm
+              remove_transaction_preserve_current_vm
+              fill_rx_unsafe_preserve_current_vm
+              copy_page_segment_unsafe_preserve_current_vm.
+      rewrite Hcureq.
+      reflexivity.
+    }
+    2: {
+      rewrite update_access_batch_preserve_regs update_ownership_batch_preserve_regs update_reg_global_update_reg.
+      (* try solve_reg_lookup. *)
+      rewrite !lookup_insert_ne; [|done].
+      rewrite get_reg_gmap_get_reg_Some.
+      rewrite /get_reg /get_reg_global /get_vm_reg_file /get_reg_files //= ?Hcureq /get_current_vm //= in HPC *.
+      rewrite <-Hcureq.
+      f_equal.
+      exists r0.
+      rewrite get_reg_gmap_get_reg_Some; auto.
+    }
+    2 : {
+      rewrite /copy_page_segment_unsafe /get_rx_pid_global /copy_from_addr_to_addr_unsafe /write_mem_segment_unsafe
+              /update_memory_global_batch /get_vm_mail_box /get_mail_boxes.
+      cbn.
+      rewrite Hpair.
+      reflexivity.
+    }
+     iDestruct ((gen_reg_update2_global PC i _ (ai ^+ 1)%f R0 i _ (encode_hvc_ret_code Succ)) with "Hσreg PC Hr0")
+      as ">[Hσreg [PC Hr0]]";try f_equal.
+    { left; done. }
+    rewrite Hcureq.
+     iFrame "Hσreg".
+    (* update page table *)
+    rewrite update_offset_PC_preserve_owned
+            update_access_batch_preserve_ownerships.
+    rewrite update_offset_PC_preserve_access.
+    rewrite (@update_ownership_batch_update_pagetable_union _ i sown spsd psd Hpsd); f_equal;eauto.
+    iDestruct ((gen_own_update_union spsd) with "HO Hσowned") as ">[Hσown' HO']"; f_equal.
+    { exact Hpsd. }
+    iFrame "Hσown'".
+    rewrite (@update_access_batch_update_pagetable_union _ i sacc ExclusiveAccess spsd psd Hpsd); f_equal;eauto.
+    iDestruct ((gen_access_update_union spsd) with "HA Hσaccess") as ">[Hσaccess' HA']";f_equal.
+    { exact Hpsd. }
+    rewrite update_ownership_batch_preserve_access update_reg_global_preserve_access remove_transaction_preserve_access
+            fill_rx_unsafe_preserve_access copy_page_segment_unsafe_preserve_access.
+    iFrame "Hσaccess'".
+    2 : {
+        by rewrite update_ownership_batch_preserve_access
+                   update_reg_global_preserve_access remove_transaction_preserve_access
+                   fill_rx_unsafe_preserve_access copy_page_segment_unsafe_preserve_access.
+    }
+    rewrite update_offset_PC_preserve_excl.
+    rewrite (@update_exclusive_batch_update_pagetable_union _ i sexcl spsd psd Hpsd); f_equal; eauto.
+    iDestruct ((gen_excl_update_union spsd) with "HE Hσexcl") as ">[Hσexcl' HE']"; f_equal.
+    { exact Hpsd. }
+    rewrite update_ownership_batch_preserve_excl update_reg_global_preserve_excl remove_transaction_preserve_excl
+            fill_rx_unsafe_preserve_excl copy_page_segment_unsafe_preserve_excl.
+    iFrame "Hσexcl'".
+    2 : {
+        by rewrite update_ownership_batch_preserve_excl update_reg_global_preserve_excl remove_transaction_preserve_excl
+                   fill_rx_unsafe_preserve_excl copy_page_segment_unsafe_preserve_excl.
+     }
+    (* update transactions *)
+    rewrite update_offset_PC_preserve_trans
+            update_access_batch_preserve_trans update_ownership_batch_preserve_trans
+            update_reg_global_preserve_trans.
+    rewrite remove_transaction_update_trans.
+    rewrite fill_rx_unsafe_preserve_trans copy_page_segment_unsafe_preserve_trans.
+    iDestruct (gen_trans_update_delete with "Hwh Htrans") as ">Htrans".
+    iFrame "Htrans".
+     (* update rx *)
+    iCombine "HRX1 HRX2" as "HRX".
+    iEval (rewrite -Hcureq) in "HRX".
+    iDestruct ((gen_rx_gmap_update_global_None (get_current_vm σ1) r1 (get_current_vm σ1) rxp) with "Hσrx2 HRX") as ">[Hσrx' [HRX1 HRX2]]".
+    rewrite update_offset_PC_preserve_rx2
+            update_access_batch_preserve_rx2
+            update_ownership_batch_preserve_rx2
+            update_reg_global_preserve_rx2
+            remove_transaction_preserve_rx2.
+    rewrite fill_rx_unsafe_update_mailbox.
+    rewrite copy_page_segment_unsafe_preserve_rx2.
+    iEval (rewrite -Hcureq /get_current_vm) in "Hσrx'".
+    rewrite -Hcureq.
+    iFrame "Hσrx'".
+    (* update mem *)
+    rewrite update_offset_PC_preserve_mem update_access_batch_preserve_mem
+            update_ownership_batch_preserve_mem update_reg_global_preserve_mem
+            remove_transaction_preserve_mem fill_rx_unsafe_preserve_mem.
+    rewrite /copy_page_segment_unsafe /copy_from_addr_to_addr_unsafe.
+    rewrite /get_tx_pid_global /get_vm_mail_box /get_mail_boxes //=.
+    rewrite -Hcureq /get_current_vm in Htx.
+    rewrite Htx.
+    rewrite /mem_region.
+    assert (Hlength: ((read_mem_segment_unsafe σ1 ptx r1)) = des).
+    {
+      rewrite /read_mem_segment_unsafe.
+      rewrite /get_mem in Hadesc.
+      apply (f_equal Z.to_nat) in Hdesl.
+      rewrite Hdesl.
+      rewrite Nat2Z.id.
+      clear Hdes Hdesl Hseq Hlendesclt Htx Hpair.
+      generalize dependent (of_pid ptx).
+      induction des; first done.
+      simpl in IHdes.
+      simpl.
+      intros.
+      rewrite /get_memory_unsafe.
+      rewrite (Hadesc 0 f a).
+      simpl.
+      f_equal.
+      rewrite /get_memory_unsafe in IHdes.
+      rewrite (IHdes (f ^+ 1)%f).
+      reflexivity.
+      intros k y1 y2 H1 H2.
+      apply Hadesc with (S k); auto.
+      reflexivity.
+      reflexivity.
+    }
+    iDestruct "HRXCont" as "[%l0 [HRXCont' %Hlen']]".
+    rewrite Hlength.
+    rewrite /write_mem_segment_unsafe //.
+    rewrite /get_rx_pid_global /get_vm_mail_box /get_mail_boxes.
+    rewrite -Hcureq in Hpair.
+    rewrite Hpair.
+    cbn.
+    iDestruct ((gen_mem_update_SepL2 (finz.seq rxp (length l0)) l0 des) with "Hσmem HRXCont'") as "Hmemupd".
+    rewrite Hlen'.
+    apply finz_seq_NoDup'.
+    pose proof last_addr_in_bound as Hbound.
+    specialize (Hbound rxp).
+    solve_finz.
+    assumption.
+    assert (Hzipeq : (zip (finz.seq rxp (length l0)) des) = (zip (finz.seq rxp (Z.to_nat 1000)) des)).
+    {
+      rewrite <-(zip_fst_snd (zip (finz.seq rxp (Z.to_nat 1000)) des)).
+      rewrite !snd_zip; auto.
+      f_equal.
+      rewrite Hlen'.
+      clear Hdes Hdesl Hseq Hadesc Hlength Hlen'.
+      generalize dependent (of_pid rxp).
+      induction des; first done.
+      cbn.
+      destruct (Z.to_nat 1000) eqn:Heqn1000; first done.
+      simpl.
+      intros f.
+      f_equal.
+      assert (Hn : n = 999).
+      lia.
+      subst n.
+      rewrite (@zip_length_le _ _ des (finz.seq (f ^+ 1)%f 999) (finz.seq (f ^+ 1)%f 1000) [(f ^+ 1000)%f]).
+      simpl in Hlendesclt.
+      rewrite IHdes.
+      reflexivity.
+      lia.
+      simpl in Hlendesclt.
+      rewrite finz_seq_length.
+      lia.
+      rewrite (finz_seq_decomposition _ 1000 _ 999).
+      f_equal.
+      simpl.
+      f_equal.
+      rewrite Unnamed_thm12.
+      rewrite Z.add_comm.
+      assert (H999_1 : Z.add (Z.of_nat 999%nat) 1%Z = 1000%Z).
+      reflexivity.
+      rewrite H999_1.
+      reflexivity.
+      lia.
+      lia.
+      lia.
+      rewrite finz_seq_length.
+      lia.
+    }
+    rewrite Hzipeq.
+    iDestruct "Hmemupd" as ">[Hmemupd1 Hmemupd2]".
+    iFrame "Hmemupd1".
+    rewrite update_offset_PC_preserve_retri update_access_batch_preserve_retri
+            update_ownership_batch_preserve_retri update_reg_global_preserve_retri.
+    iDestruct ((gen_retri_update_delete wh) with "Hwhf Hrcv") as ">Hrcv".
+    rewrite remove_transaction_update_retri.
+    rewrite fill_rx_unsafe_preserve_receivers.
+    assert (Htemp : ∀ σ l, get_retri_gmap (update_memory_global_batch σ l) = get_retri_gmap σ). f_equal.
+    rewrite Htemp; clear Htemp.
+    iFrame "Hrcv".
+    iCombine "Hpool Hσhp" as "Hhp".
+    iDestruct ((@gen_hpool_update_union _ _ σ1 sh 1 wh) with "Hhp") as ">[Hσhp' Hpool']".
+    {
+      rewrite /get_hpool_gset.
+      rewrite /get_fresh_handles in Hpool.
+      intros contra.
+      assert (contra' : wh ∉ dom (gset handle) (get_transactions σ1).1).
+      {
+        symmetry in Hdisj.
+        rewrite ->elem_of_disjoint in Hdisj.
+        specialize (Hdisj wh contra).
+        auto.
+      }
+      apply contra'.
+      apply elem_of_dom.
+      exists t.
+      auto.
+    }
+    rewrite update_offset_PC_preserve_hpool update_access_batch_preserve_hpool
+            update_ownership_batch_preserve_hpool update_reg_global_preserve_hpool.
+    rewrite remove_transaction_update_hpool.
+    rewrite fill_rx_unsafe_preserve_hpool.
+    assert (Htemp : ∀ σ l, get_hpool_gset (update_memory_global_batch σ l) = get_hpool_gset σ). f_equal.
+    rewrite Htemp; clear Htemp.
+    iFrame "Hσhp'".
+    iSplitR.
+    iPureIntro.
+    rewrite update_offset_PC_preserve_trans'
+            update_access_batch_preserve_trans'
+            update_ownership_batch_preserve_trans'
+            update_reg_global_preserve_trans'.
+    rewrite /get_transactions.
+    cbn.
+    split.
+    rewrite dom_delete.
+    rewrite disjoint_union_r.
+    split.
+    apply disjoint_difference_l2; auto.
+    apply disjoint_difference_l1; auto.
+    apply map_Forall_delete; auto.
+    iApply "HΦ".
+    rewrite Hlen'.
+    by iFrame.
+Qed.
+
+Lemma hvc_retrieve_lend_nz {wi sown sacc pi sexcl i j des ptx rxp l} {spsd: gset PID}
+      ai r0 r1 wh wf (psd: list PID) :
+  (* the current instruction is hvc *)
+  (* the decoding of wi is correct *)
+  decode_instruction wi = Some(Hvc) ->
+  (* the instruction is in page pi *)
+  addr_in_page ai pi ->
+  (* the decoding of R0 is FFA_DONATE *)
+  decode_hvc_func r0 = Some(Retrieve) ->
+  (* pi page in spsd is accessible for VM i *)
+  pi ∈ sacc ->
+  (* spsd is the gset of all to-be-donated pages *)
+  spsd = (list_to_set psd) ->
+  spsd ## sacc ->
+  spsd ## sown ->
+  spsd ## sexcl ->
+  (finz.to_z l) = (Z.of_nat (length psd)) ->
+  des = ([of_imm (encode_vmid j); wf; wh; l; of_imm (encode_vmid i)] ++ map of_pid psd) ->
+  (finz.to_z r1) = (Z.of_nat (length des)) ->
+  seq_in_page (of_pid ptx) (length des) ptx ->
+  {SS{{ ▷(PC @@ i ->r ai) ∗ ▷ ai ->a wi ∗ ▷ A@i:={1}[sacc]
+  ∗ ▷ (R0 @@ i ->r r0) ∗ ▷ wh ->re false
+  ∗ ▷ (R1 @@ i ->r r1) ∗ ▷ wh ->t{1}(j, wf, i, psd, Lending)
+  ∗ ▷ O@i:={1}[sown] ∗ ▷ E@i:={1}[sexcl] ∗ ▷ TX@ i := ptx
+  ∗ ▷ mem_region des ptx ∗ ▷ RX@ i :=( rxp !) ∗ ▷ (∃l, mem_region l rxp ∗ ⌜ length l = length des ⌝)}}}
+   ExecI @ i {{{ RET ExecI ; PC @@ i ->r (ai ^+ 1)%f ∗ ai ->a wi
+  ∗ O@i:={1}[(sown)] ∗ E@i:={1}[(sexcl ∪ spsd)] ∗ A@i:={1}[(sacc ∪ spsd)]
+  ∗ R0 @@ i ->r (encode_hvc_ret_code Succ) ∗ R1 @@ i ->r r1 ∗ wh ->t{1}(j, wf, i, psd, Lending)
   ∗ wh ->re true ∗ TX@ i := ptx ∗ RX@ i :=( rxp ! r1, i)
   ∗ mem_region des ptx ∗ mem_region des rxp }}}.
 Proof.
@@ -88,7 +452,24 @@ Proof.
     rewrite /get_tx_pid_global Hcureq Htx in Heqc2.
     rewrite (@transaction_retrieve_descriptor_valid j wh wf l psd σ1 des ptx) /= in Heqc2; eauto.    
     2: { rewrite Hcureq; auto. }
-    rewrite Htrans /= Hcureq in Heqc2.    
+    rewrite Htrans /= in Heqc2.
+    rewrite /transfer_msg Hcureq in Heqc2.
+    rewrite /transfer_msg_unsafe Hr1ps in Heqc2.
+    rewrite /fill_rx in Heqc2.
+    assert (Htemp : ∀ σ t r r1 i, get_vm_mail_box (copy_page_segment_unsafe σ t r r1) i =
+                                  get_vm_mail_box σ i).
+    f_equal.
+    rewrite Htemp in Heqc2; clear Htemp.
+    rewrite /get_vm_mail_box /get_mail_boxes in Htx Hrx2.
+    pose proof (surjective_pairing (σ1.1.1.1.1.2 !!! i)) as Hpair.
+    rewrite (surjective_pairing (σ1.1.1.1.1.2 !!! i).2) in Hpair.
+    rewrite Htx Hrx1 Hrx2 in Hpair.
+    rewrite /get_vm_mail_box /get_mail_boxes in Heqc2.
+    rewrite Hpair // in Heqc2.
+    simpl in Heqc2.
+    rewrite fill_rx_unsafe_preserve_current_vm in Heqc2.
+    rewrite copy_page_segment_unsafe_preserve_current_vm in Heqc2.
+    rewrite Hcureq in Heqc2.
     assert (Hcheck : (i =? i)%nat = true).
     { by apply <- Nat.eqb_eq. }
     rewrite Hcheck in Heqc2.
@@ -98,52 +479,57 @@ Proof.
     inversion Hretri1 as [Hretri1'].
     rewrite -Hretri1' //= in Hretri2.
     rewrite Hretri2 //= /transaction_write_rx /transaction_to_list_words /transaction_to_transaction_descriptor in Heqc2.
-    pose proof (finz_of_z_to_z word_size l) as Htemp.
-    rewrite Hlenl in Htemp.
-    rewrite /transfer_msg /transfer_msg_unsafe Hr1ps //= /get_current_vm //= /get_vm_mail_box /get_mail_boxes //in Heqc2.
-    rewrite /get_vm_mail_box /get_mail_boxes in Htx Hrx2.
-    pose proof (surjective_pairing (σ1.1.1.1.1.2 !!! i)) as Hpair.
-    rewrite (surjective_pairing (σ1.1.1.1.1.2 !!! i).2) in Hpair.
-    rewrite Htx Hrx1 Hrx2 in Hpair.
-    rewrite //= /fill_rx /get_vm_mail_box /get_mail_boxes // /get_mail_boxes // in Heqc2.
-    rewrite Hpair //= in Heqc2.
-    destruct HstepP; subst m2 σ2; subst c2; simpl.
+    assert (Htemp :
+              c2.2 =
+              update_incr_PC
+                (update_access_batch
+                   (update_reg (fill_rx_unsafe
+                                  (copy_page_segment_unsafe (get_reg_files σ1,
+                                                             get_mail_boxes σ1,
+                                                             get_page_tables σ1, i,
+                                                             get_mem σ1,
+                                                             (<[wh := (j, wf, true, i, psd, Lending)]> (get_transactions σ1).1, (get_transactions σ1).2)) (get_tx_pid_global σ1 i)
+                                                            (get_rx_pid_global σ1 i) r1) r1 i i ptx rxp) R0
+                               (encode_hvc_ret_code Succ)) psd ExclusiveAccess)).
+    {
+      rewrite Heqc2 //=.
+    }
+    destruct c2 as [c21 c22].
+    simpl in Heqc2.
+    simpl in Htemp.
+    destruct HstepP; subst m2 σ2; subst c22.
+    inversion Heqc2 as [Htemp].
+    subst c21; simpl.
     rewrite /gen_vm_interp /update_incr_PC /update_reg.
-    rewrite_reg_pc.
-    rewrite_reg_global.
-    rewrite_access_all.
-    rewrite_ownership_all.
-    rewrite_reg_global.
-    rewrite fill_rx_unsafe_preserve_current_vm.
-    rewrite copy_page_segment_unsafe_preserve_current_vm.
+    rewrite update_offset_PC_preserve_hpool update_access_batch_preserve_hpool
+            update_reg_global_preserve_hpool fill_rx_unsafe_preserve_hpool
+            copy_page_segment_unsafe_preserve_hpool.
     iFrame "Hσhp".
-    rewrite fill_rx_unsafe_preserve_tx.
+    rewrite update_offset_PC_preserve_tx update_access_batch_preserve_tx
+            update_reg_global_preserve_tx fill_rx_unsafe_preserve_tx.
     2 : {
       rewrite /get_tx_pid_global /get_vm_mail_box //= /get_mail_boxes.
     }
     rewrite copy_page_segment_unsafe_preserve_tx.
     rewrite /get_tx_agree.
     iFrame "Hσtx".
-    rewrite fill_rx_unsafe_preserve_receivers copy_page_segment_unsafe_preserve_receivers.
-    rewrite fill_rx_unsafe_preserve_trans copy_page_segment_unsafe_preserve_trans.
-    rewrite fill_rx_unsafe_preserve_mem.
+    rewrite update_offset_PC_preserve_current_vm update_access_batch_preserve_current_vm
+            update_reg_global_preserve_current_vm fill_rx_unsafe_preserve_current_vm
+            copy_page_segment_unsafe_preserve_current_vm.
+    cbn.
     rewrite Hcureq.
-    rewrite /get_current_vm.
-    iSimpl.
     iFrame "Hcur".
+    rewrite update_offset_PC_preserve_rx1 update_access_batch_preserve_rx1
+            update_reg_global_preserve_rx1.
     rewrite fill_rx_unsafe_preserve_rx1.
      2 : {
        rewrite /get_rx_pid_global /get_vm_mail_box /get_mail_boxes //=.
      }
      rewrite copy_page_segment_unsafe_preserve_rx1.
      iFrame "Hσrx1".
-     rewrite fill_rx_unsafe_update_mailbox.
-     rewrite copy_page_segment_unsafe_preserve_rx2.
-     rewrite update_access_batch_preserve_ownerships.
-
     (* update regs *)
     rewrite (update_offset_PC_update_PC1 _ i ai 1).
-    rewrite update_access_batch_preserve_regs update_ownership_batch_preserve_regs update_reg_global_update_reg
+    rewrite update_access_batch_preserve_regs update_reg_global_update_reg
              fill_rx_unsafe_preserve_regs copy_page_segment_unsafe_preserve_regs; try solve_reg_lookup.
     2 : {
       exists r0.
@@ -155,7 +541,7 @@ Proof.
       f_equal.
     }
     2:{
-      rewrite update_access_batch_preserve_regs update_ownership_batch_preserve_regs update_reg_global_update_reg.
+      rewrite update_access_batch_preserve_regs update_reg_global_update_reg.
       (* try solve_reg_lookup. *)
       rewrite !lookup_insert_ne; [|done].
       rewrite get_reg_gmap_get_reg_Some.
@@ -169,190 +555,194 @@ Proof.
       as ">[Hσreg [PC Hr0]]";try f_equal.
     { left;done. }
      iFrame "Hσreg".
-      (* update page table *)
-     rewrite (@update_ownership_batch_update_pagetable_union _ i sown spsd psd Hpsd); f_equal;eauto.
-     iDestruct ((gen_own_update_union spsd) with "HO Hσowned") as ">[Hσown' HO']"; f_equal.
+    (* update page table *)
+    rewrite update_offset_PC_preserve_owned update_access_batch_preserve_ownerships
+            update_reg_global_preserve_owned fill_rx_unsafe_preserve_owned copy_page_segment_unsafe_preserve_owned.    
+    iFrame "Hσowned".
+    rewrite update_offset_PC_preserve_access.
+    rewrite (@update_access_batch_update_pagetable_union _ i sacc ExclusiveAccess spsd psd Hpsd); f_equal;eauto.
+    iDestruct ((gen_access_update_union spsd) with "HA Hσaccess") as ">[Hσaccess' HA']";f_equal.
+    {exact Hpsd. }
+    rewrite update_reg_global_preserve_access
+    fill_rx_unsafe_preserve_access copy_page_segment_unsafe_preserve_access.
+    iFrame "Hσaccess'".
+    rewrite update_offset_PC_preserve_excl.
+    rewrite (@update_exclusive_batch_update_pagetable_union _ i sexcl spsd psd Hpsd);f_equal; eauto.
+    iDestruct ((gen_excl_update_union spsd) with "HE Hσexcl") as ">[Hσexcl' HE']"; f_equal.
     { exact Hpsd. }
-     iFrame "Hσown'".
-     rewrite (@update_access_batch_update_pagetable_union _ i sacc ExclusiveAccess spsd psd Hpsd); f_equal;eauto.
-     iDestruct ((gen_access_update_union spsd) with "HA Hσaccess") as ">[Hσaccess' HA']";f_equal.
-     {exact Hpsd. }
-     rewrite update_ownership_batch_preserve_access update_reg_global_preserve_access
-             fill_rx_unsafe_preserve_access copy_page_segment_unsafe_preserve_access.
-     iFrame "Hσaccess'".
-     2 : {
-       by rewrite update_ownership_batch_preserve_access update_reg_global_preserve_access
-               fill_rx_unsafe_preserve_access copy_page_segment_unsafe_preserve_access.
-     }
-     rewrite (@update_exclusive_batch_update_pagetable_union _ i sexcl spsd psd Hpsd);f_equal; eauto.
-     iDestruct ((gen_excl_update_union spsd) with "HE Hσexcl") as ">[Hσexcl' HE']"; f_equal.
-     { exact Hpsd. }
-     rewrite update_ownership_batch_preserve_excl update_reg_global_preserve_excl
-             fill_rx_unsafe_preserve_excl copy_page_segment_unsafe_preserve_excl.
-     iFrame "Hσexcl'".
-     2 : {
-       by rewrite update_ownership_batch_preserve_excl update_reg_global_preserve_excl
-               fill_rx_unsafe_preserve_excl copy_page_segment_unsafe_preserve_excl.
-     }
-
-     (* update transactions *)
-     rewrite <-Hcureq.
-     rewrite (@toggle_transaction_unsafe_preserve_trans _ _ b).
-     2 : {
-       rewrite Hcureq.
-       assumption.
-     }
-     iFrame "Htrans".
-     (* update retri *)
-     assert (HTemp : (get_retri_gmap σ1) !! wh = Some false).
-     {
-       rewrite /get_retri_gmap /get_transactions_gmap.
-       apply elem_of_list_to_map_1'.
-       intros y Hy.
-       apply elem_of_list_In in Hy.
-       apply in_map_iff in Hy.
-       destruct Hy as [y' [Hy1 Hy2]].
-       inversion Hy1; subst; clear Hy1.
-       apply elem_of_list_In in Hy2.
-       apply elem_of_map_to_list' in Hy2.
-       rewrite Hretri1'' in Hy2.
-       inversion Hy2; subst; clear Hy2.
-       reflexivity.
-       apply elem_of_list_In.
-       apply in_map_iff.
-       exists (wh, t).
-       split.
-       inversion Hretri1'; subst.
-       reflexivity.
-       apply elem_of_list_In.
-       apply elem_of_map_to_list'.
-       simpl.
-       assumption.
-     }
-     iDestruct ((@gen_retri_update _ _ _ false true wh HTemp) with "Hwhf Hrcv") as ">[Hrcv' Hwhf']".
-     assert (HTemp' : σ1.1.1.1.1.2 = get_mail_boxes σ1).
-     {
-       rewrite /get_mail_boxes.
-       reflexivity.
-     }
-     rewrite HTemp'.
-     rewrite <-(@get_retri_gmap_to_get_transaction σ1 wh j wf true (get_current_vm σ1) psd Donation).
-     iFrame "Hrcv'".
-     (* update rx *)
-     iCombine "HRX1 HRX2" as "HRX".
-     iDestruct ((gen_rx_gmap_update_global_None (get_current_vm σ1) r1 (get_current_vm σ1) rxp) with "Hσrx2 HRX") as ">[Hσrx' [HRX1 HRX2]]".
-     iFrame "Hσrx'".
-     (* update mem *)
-     rewrite /copy_page_segment_unsafe /copy_from_addr_to_addr_unsafe.
-     rewrite /get_tx_pid_global /get_vm_mail_box /get_mail_boxes //=.
-     rewrite <-Hcureq in Htx.
-     rewrite Htx.
-     rewrite /mem_region.
-     assert (Hlength: ((read_mem_segment_unsafe
-                          (get_reg_files σ1, σ1.1.1.1.1.2, get_page_tables σ1, get_current_vm σ1, get_mem σ1,
-                           (<[wh := (j, wf, true, get_current_vm σ1, psd, Donation)]> (get_transactions σ1).1,
-                            (get_transactions σ1).2)) ptx r1)) = des).
-     {
-       rewrite /read_mem_segment_unsafe.
-       rewrite /get_mem in Hadesc.
-       apply (f_equal Z.to_nat) in Hdesl.
-       rewrite Hdesl.
-       rewrite Nat2Z.id.
-       clear Hdes Hdesl Hseq Hlendesclt Htx Hpair.
-       generalize dependent (of_pid ptx).
-       induction des; first done.
-       simpl in IHdes.
-       simpl.
-       intros.
-       rewrite /get_memory_unsafe.
-       rewrite (Hadesc 0 f a).
-       simpl.
-       f_equal.
-       rewrite /get_memory_unsafe in IHdes.
-       rewrite (IHdes (f ^+ 1)%f).
-       reflexivity.
-       intros k y1 y2 H1 H2.
-       apply Hadesc with (S k); auto.
-       reflexivity.
-       reflexivity.
-     }
-     iDestruct "HRXCont" as "[%l0 [HRXCont' %Hlen']]".
-     rewrite Hlength.
-     rewrite /write_mem_segment_unsafe //.
-     rewrite /get_rx_pid_global /get_vm_mail_box /get_mail_boxes.
-     assert (Heq1 : (get_reg_files σ1, σ1.1.1.1.1.2, get_page_tables σ1, get_current_vm σ1, 
-                     get_mem σ1,
-                     (<[wh := (j, wf, true, get_current_vm σ1, psd, Donation)]> (get_transactions σ1).1,
-                      (get_transactions σ1).2)).1.1.1.1.2 = σ1.1.1.1.1.2).
-     auto.
-     rewrite Heq1.
-     rewrite <-Hcureq in Hpair.
-     rewrite Hpair.
-     cbn.
-     iDestruct ((gen_mem_update_SepL2 (finz.seq rxp (length l0)) l0 des) with "Hσmem HRXCont'") as "Hmemupd".
-     rewrite Hlen'.
-     apply finz_seq_NoDup'.
-     pose proof last_addr_in_bound as Hbound.
-     specialize (Hbound rxp).
-     solve_finz.
-     assumption.
-     assert (Hzipeq : (zip (finz.seq rxp (length l0)) des) = (zip (finz.seq rxp (Z.to_nat 1000)) des)).
-     {
-       rewrite <-(zip_fst_snd (zip (finz.seq rxp (Z.to_nat 1000)) des)).
-       rewrite !snd_zip; auto.
-       f_equal.
-       rewrite Hlen'.
-       clear Hdes Hdesl Hseq Hadesc Hlength Hlen'.
-       generalize dependent (of_pid rxp).
-       induction des; first done.
-       cbn.
-       destruct (Z.to_nat 1000) eqn:Heqn1000; first done.
-       simpl.
-       intros f.
-       f_equal.
-       assert (Hn : n = 999).
-       lia.
-       subst n.
-       rewrite (@zip_length_le _ _ des (finz.seq (f ^+ 1)%f 999) (finz.seq (f ^+ 1)%f 1000) [(f ^+ 1000)%f]).
-       simpl in Hlendesclt.
-       rewrite IHdes.
-       reflexivity.
-       lia.
-       simpl in Hlendesclt.
-       rewrite finz_seq_length.
-       lia.
-       rewrite (finz_seq_decomposition _ 1000 _ 999).
-       f_equal.
-       simpl.
-       f_equal.
-       rewrite Unnamed_thm12.
-       rewrite Z.add_comm.
-       assert (H999_1 : Z.add (Z.of_nat 999%nat) 1%Z = 1000%Z).
-       reflexivity.
-       rewrite H999_1.
-       reflexivity.
-       lia.
-       lia.
-       lia.
-       rewrite finz_seq_length.
-       lia.
-     }
-     rewrite Hzipeq.
-     iDestruct "Hmemupd" as ">[Hmemupd1 Hmemupd2]".
-     iFrame "Hmemupd1".
-          iSplitR.
-     iPureIntro.
-     rewrite dom_insert_lookup_L; eauto.
-     split; [set_solver|].
-     apply map_Forall_insert_2; auto.
-     simpl.
-     rewrite <-Hlenl.
-     destruct (finz_spec word_size l) as [H _].
-     rewrite ->(reflect_iff _ _ (Z.ltb_spec0 l word_size)) in H.
-     assumption.
-     iApply "HΦ".
-     rewrite Hlen'.
-     by iFrame.
+    rewrite update_reg_global_preserve_excl
+    fill_rx_unsafe_preserve_excl copy_page_segment_unsafe_preserve_excl.
+    iFrame "Hσexcl'".
+    (* update transactions *)
+    rewrite <-Hcureq.
+    rewrite update_offset_PC_preserve_trans update_access_batch_preserve_trans
+            update_reg_global_preserve_trans fill_rx_unsafe_preserve_trans copy_page_segment_unsafe_preserve_trans.    
+    rewrite (@toggle_transaction_unsafe_preserve_trans _ _ b).
+    2 : {
+      rewrite Hcureq.
+      assumption.
+    }
+    iFrame "Htrans".
+    (* update retri *)
+    assert (HTemp : (get_retri_gmap σ1) !! wh = Some false).
+    {
+      rewrite /get_retri_gmap /get_transactions_gmap.
+      apply elem_of_list_to_map_1'.
+      intros y Hy.
+      apply elem_of_list_In in Hy.
+      apply in_map_iff in Hy.
+      destruct Hy as [y' [Hy1 Hy2]].
+      inversion Hy1; subst; clear Hy1.
+      apply elem_of_list_In in Hy2.
+      apply elem_of_map_to_list' in Hy2.
+      rewrite Hretri1'' in Hy2.
+      inversion Hy2; subst; clear Hy2.
+      reflexivity.
+      apply elem_of_list_In.
+      apply in_map_iff.
+      exists (wh, t).
+      split.
+      inversion Hretri1'; subst.
+      reflexivity.
+      apply elem_of_list_In.
+      apply elem_of_map_to_list'.
+      simpl.
+      assumption.
+    }
+    iDestruct ((@gen_retri_update _ _ _ false true wh HTemp) with "Hwhf Hrcv") as ">[Hrcv' Hwhf']".
+    assert (HTemp' : σ1.1.1.1.1.2 = get_mail_boxes σ1).
+    {
+      rewrite /get_mail_boxes.
+      reflexivity.
+    }
+    rewrite update_offset_PC_preserve_retri update_access_batch_preserve_retri
+    update_reg_global_preserve_retri fill_rx_unsafe_preserve_receivers
+    copy_page_segment_unsafe_preserve_receivers.
+    rewrite <-(@get_retri_gmap_to_get_transaction σ1 wh j wf true (get_current_vm σ1) psd Lending).
+    iFrame "Hrcv'".
+    (* update rx *)
+    iCombine "HRX1 HRX2" as "HRX".
+    rewrite update_offset_PC_preserve_rx2 update_access_batch_preserve_rx2
+            update_reg_global_preserve_rx2.
+    iDestruct ((gen_rx_gmap_update_global_None (get_current_vm σ1) r1 (get_current_vm σ1) rxp) with "Hσrx2 HRX") as ">[Hσrx' [HRX1 HRX2]]".
+    rewrite fill_rx_unsafe_update_mailbox.
+    iFrame "Hσrx'".
+    (* update mem *)
+    rewrite update_offset_PC_preserve_mem update_access_batch_preserve_mem
+            update_reg_global_preserve_mem fill_rx_unsafe_preserve_mem.
+    rewrite /copy_page_segment_unsafe /copy_from_addr_to_addr_unsafe.
+    rewrite /get_tx_pid_global /get_vm_mail_box /get_mail_boxes //=.
+    rewrite <-Hcureq in Htx.
+    rewrite Htx.
+    rewrite /mem_region.
+    assert (Hlength: ((read_mem_segment_unsafe
+                         (get_reg_files σ1, σ1.1.1.1.1.2, get_page_tables σ1, get_current_vm σ1, get_mem σ1,
+                          (<[wh := (j, wf, true, get_current_vm σ1, psd, Lending)]> (get_transactions σ1).1,
+                           (get_transactions σ1).2)) ptx r1)) = des).
+    {
+      rewrite /read_mem_segment_unsafe.
+      rewrite /get_mem in Hadesc.
+      apply (f_equal Z.to_nat) in Hdesl.
+      rewrite Hdesl.
+      rewrite Nat2Z.id.
+      clear Hdes Hdesl Hseq Hlendesclt Htx Hpair.
+      generalize dependent (of_pid ptx).
+      induction des; first done.
+      simpl in IHdes.
+      simpl.
+      intros.
+      rewrite /get_memory_unsafe.
+      rewrite (Hadesc 0 f a).
+      simpl.
+      f_equal.
+      rewrite /get_memory_unsafe in IHdes.
+      rewrite (IHdes (f ^+ 1)%f).
+      reflexivity.
+      intros k y1 y2 H1 H2.
+      apply Hadesc with (S k); auto.
+      reflexivity.
+      reflexivity.
+    }
+    iDestruct "HRXCont" as "[%l0 [HRXCont' %Hlen']]".
+    rewrite Hlength.
+    rewrite /write_mem_segment_unsafe //.
+    rewrite /get_rx_pid_global /get_vm_mail_box /get_mail_boxes.
+    assert (Heq1 : (get_reg_files σ1, σ1.1.1.1.1.2, get_page_tables σ1, get_current_vm σ1, 
+                    get_mem σ1,
+                    (<[wh := (j, wf, true, get_current_vm σ1, psd, Lending)]> (get_transactions σ1).1,
+                     (get_transactions σ1).2)).1.1.1.1.2 = σ1.1.1.1.1.2).
+    auto.
+    rewrite <-Hcureq in Hpair.
+    rewrite Hpair.
+    cbn.
+    iDestruct ((gen_mem_update_SepL2 (finz.seq rxp (length l0)) l0 des) with "Hσmem HRXCont'") as "Hmemupd".
+    rewrite Hlen'.
+    apply finz_seq_NoDup'.
+    pose proof last_addr_in_bound as Hbound.
+    specialize (Hbound rxp).
+    solve_finz.
+    assumption.
+    assert (Hzipeq : (zip (finz.seq rxp (length l0)) des) = (zip (finz.seq rxp (Z.to_nat 1000)) des)).
+    {
+      rewrite <-(zip_fst_snd (zip (finz.seq rxp (Z.to_nat 1000)) des)).
+      rewrite !snd_zip; auto.
+      f_equal.
+      rewrite Hlen'.
+      clear Hdes Hdesl Hseq Hadesc Hlength Hlen'.
+      generalize dependent (of_pid rxp).
+      induction des; first done.
+      cbn.
+      destruct (Z.to_nat 1000) eqn:Heqn1000; first done.
+      simpl.
+      intros f.
+      f_equal.
+      assert (Hn : n = 999).
+      lia.
+      subst n.
+      rewrite (@zip_length_le _ _ des (finz.seq (f ^+ 1)%f 999) (finz.seq (f ^+ 1)%f 1000) [(f ^+ 1000)%f]).
+      simpl in Hlendesclt.
+      rewrite IHdes.
+      reflexivity.
+      lia.
+      simpl in Hlendesclt.
+      rewrite finz_seq_length.
+      lia.
+      rewrite (finz_seq_decomposition _ 1000 _ 999).
+      f_equal.
+      simpl.
+      f_equal.
+      rewrite Unnamed_thm12.
+      rewrite Z.add_comm.
+      assert (H999_1 : Z.add (Z.of_nat 999%nat) 1%Z = 1000%Z).
+      reflexivity.
+      rewrite H999_1.
+      reflexivity.
+      lia.
+      lia.
+      lia.
+      rewrite finz_seq_length.
+      lia.
+    }
+    rewrite Hzipeq.
+    iDestruct "Hmemupd" as ">[Hmemupd1 Hmemupd2]".
+    iFrame "Hmemupd1".
+    iSplitR.
+    iPureIntro.
+    rewrite update_offset_PC_preserve_trans'
+            update_access_batch_preserve_trans'
+            update_reg_global_preserve_trans'.
+    cbn.
+    rewrite dom_insert_lookup_L; eauto.
+    split; [set_solver|].
+    apply map_Forall_insert_2; auto.
+    simpl.
+    rewrite <-Hlenl.
+    destruct (finz_spec word_size l) as [H _].
+    rewrite ->(reflect_iff _ _ (Z.ltb_spec0 l word_size)) in H.
+    assumption.
+    iApply "HΦ".
+    rewrite Hlen'.
+    by iFrame.
 Qed.
 
 End retrieve.
